Add UBFM to ARM model and make other improvements
The main enhancement is to add the general case of the UBFM (unsigned
bitfield move) instruction to the formal ARM model. The basic left and
right shifts are now done properly as special cases: although there
are still pseudo-instructions for them at the shallow embedding level,
the decoding function gives the UBFM form that is proved equivalent
later in the simulation process.

This update also fills out and regularizes the existing suite of basic
operations in a natural way by adding ASRV, BIC, BICS and RORV, as
well as calling out a few additional aliases. Finally, it fixes an
error in decoding of a couple of instruction classes where the
decision over the interpretation of register 31 as the zero register
or stack pointer was insufficiently nuanced (basically, it depends
in these cases on whether it is an "S"-suffixed flag-setting form).

arm/proofs/instruction.ml
@@ -615,7 +615,7 @@ let arm_ADC = define
     \s. let m = read Rm s
         and n = read Rn s
         and c = bitval(read CF s) in
-        let d = word_add (word_add m n) (word c) in
+        let d:N word = word_add (word_add m n) (word c) in
         (Rd := d) s`;;
 
 let arm_ADCS = define
@@ -623,7 +623,7 @@ let arm_ADCS = define
     \s. let m = read Rm s
         and n = read Rn s
         and c = bitval(read CF s) in
-        let d = word_add (word_add m n) (word c) in
+        let d:N word = word_add (word_add m n) (word c) in
         (Rd := d ,,
          NF := (ival d < &0) ,,
          ZF := (val d = 0) ,,
@@ -634,14 +634,14 @@ let arm_ADD = define
  `arm_ADD Rd Rm Rn =
     \s. let m = read Rm s
         and n = read Rn s in
-        let d = word_add m n in
+        let d:N word = word_add m n in
         (Rd := d) s`;;
 
 let arm_ADDS = define
  `arm_ADDS Rd Rm Rn =
     \s. let m = read Rm s
         and n = read Rn s in
-        let d = word_add m n in
+        let d:N word = word_add m n in
         (Rd := d ,,
          NF := (ival d < &0) ,,
          ZF := (val d = 0) ,,
@@ -652,19 +652,26 @@ let arm_AND = define
  `arm_AND Rd Rm Rn =
     \s. let m = read Rm s
         and n = read Rn s in
-        let d = word_and m n in
+        let d:N word = word_and m n in
         (Rd := d) s`;;
 
 let arm_ANDS = define
  `arm_ANDS Rd Rm Rn =
     \s. let m = read Rm s
         and n = read Rn s in
-        let d = word_and m n in
+        let d:N word = word_and m n in
         (Rd := d ,,
          NF := (ival d < &0) ,,
          ZF := (val d = 0) ,,
          CF := F ,,
          VF := F) s`;;
+
+let arm_ASRV = define
+ `arm_ASRV Rd Rm Rn =
+    \s. let m = read Rm s
+        and n = read Rn s in
+        let d:N word = word_jshr m n in
+        (Rd := d) s`;;
 
 (*** For unconditional branch the offset is encoded as a 26-bit word   ***)
 (*** This is turned into a 28-bit word when multiplied by 4, then sx   ***)
@@ -673,6 +680,24 @@ let arm_ANDS = define
 let arm_B = define
  `arm_B (off:28 word) =
     \s. (PC := word_add (word_sub (read PC s) (word 4)) (word_sx off)) s`;;
+
+let arm_BIC = define
+ `arm_BIC Rd Rm Rn =
+    \s. let m = read Rm s
+        and n = read Rn s in
+        let d:N word = word_and m (word_not n) in
+        (Rd := d) s`;;
+
+let arm_BICS = define
+ `arm_BICS Rd Rm Rn =
+    \s. let m = read Rm s
+        and n = read Rn s in
+        let d:N word = word_and m (word_not n) in
+        (Rd := d ,,
+         NF := (ival d < &0) ,,
+         ZF := (val d = 0) ,,
+         CF := F ,,
+         VF := F) s`;;
 
 (*** As with x86, we have relative and absolute versions of branch & link ***)
 (*** The absolute one gives a natural way of handling linker-insertions.  ***)
@@ -743,48 +768,41 @@ let arm_EON = define
  `arm_EON Rd Rm Rn =
     \s. let m = read Rm s
         and n = read Rn s in
-        let d = word_xor m (word_not n) in
+        let d:N word = word_xor m (word_not n) in
         (Rd := d) s`;;
 
 let arm_EOR = define
  `arm_EOR Rd Rm Rn =
     \s. let m = read Rm s
         and n = read Rn s in
-        let d = word_xor m n in
+        let d:N word = word_xor m n in
         (Rd := d) s`;;
 
-(*** We force the shift count to be of the same word type; in practice
- *** it would be fine to use 6-bit immediates for 64-bit main values,
- *** which is all we currently use
+(*** The lsb argument is forced modulo the wordsize here, but that should
+ *** happen implicitly from the size of the immediate when using the decoder.
  ***)
 
 let arm_EXTR = define
  `arm_EXTR Rd Rn Rm lsb =
     \s. let n:N word = read Rn s
         and m:N word = read Rm s
-        and l = val(read lsb s:N word) MOD dimindex(:N) in
+        and l = lsb MOD dimindex(:N) in
         let concat:(N tybit0)word = word_join n m in
         let d:N word = word_subword concat (l,dimindex(:N)) in
         (Rd := d) s`;;
-
-(*** Note that the shift behaviours in the LSLV and LSRV docs
- *** exactly match the word_jshl and word_jushr with a masking;
- *** the English text about "remainder on dividing" is ambiguous
- *** but it's quite explicitly treated as unsigned in pseudocode
- ***)
 
 let arm_LSLV = define
  `arm_LSLV Rd Rm Rn =
     \s. let m = read Rm s
         and n = read Rn s in
-        let d = word_jshl m n in
+        let d:N word = word_jshl m n in
         (Rd := d) s`;;
 
 let arm_LSRV = define
  `arm_LSRV Rd Rm Rn =
     \s. let m = read Rm s
         and n = read Rn s in
-        let d = word_jushr m n in
+        let d:N word = word_jushr m n in
         (Rd := d) s`;;
 
 let arm_MADD = define
@@ -819,14 +837,14 @@ let arm_ORN = define
  `arm_ORN Rd Rm Rn =
     \s. let m = read Rm s
         and n = read Rn s in
-        let d = word_or m (word_not n) in
+        let d:N word = word_or m (word_not n) in
         (Rd := d) s`;;
 
 let arm_ORR = define
  `arm_ORR Rd Rm Rn =
     \s. let m = read Rm s
         and n = read Rn s in
-        let d = word_or m n in
+        let d:N word = word_or m n in
         (Rd := d) s`;;
 
 (*** The default RET uses X30. ***)
@@ -834,6 +852,13 @@ let arm_ORR = define
 let arm_RET = define
  `arm_RET Rn =
     \s. (PC := read Rn s) s`;;
+
+let arm_RORV = define
+ `arm_RORV Rd Rm Rn =
+    \s. let m = read Rm s
+        and n = read Rn s in
+        let d:N word = word_jror m n in
+        (Rd := d) s`;;
 
 (*** Note that the carry flag is inverted for subtractions ***)
 (*** Flag set means no borrow, flag clear means borrow.    ***)
@@ -844,7 +869,7 @@ let arm_SBC = define
     \s. let m = read Rm s
         and n = read Rn s
         and c = bitval(~read CF s) in
-        let d = word_sub m (word_add n (word c)) in
+        let d:N word = word_sub m (word_add n (word c)) in
         (Rd := d) s`;;
 
 let arm_SBCS = define
@@ -852,7 +877,7 @@ let arm_SBCS = define
     \s. let m = read Rm s
         and n = read Rn s
         and c = bitval(~read CF s) in
-        let d = word_sub m (word_add n (word c)) in
+        let d:N word = word_sub m (word_add n (word c)) in
         (Rd := d ,,
          NF := (ival d < &0) ,,
          ZF := (val d = 0) ,,
@@ -863,19 +888,27 @@ let arm_SUB = define
  `arm_SUB Rd Rm Rn =
     \s. let m = read Rm s
         and n = read Rn s in
-        let d = word_sub m n in
+        let d:N word = word_sub m n in
         (Rd := d) s`;;
 
 let arm_SUBS = define
  `arm_SUBS Rd Rm Rn =
     \s. let m = read Rm s
         and n = read Rn s in
-        let d = word_sub m n in
+        let d:N word = word_sub m n in
         (Rd := d ,,
          NF := (ival d < &0) ,,
          ZF := (val d = 0) ,,
          CF := (&(val m) - &(val n):int = &(val d)) ,,
          VF := ~(ival m - ival n = ival d)) s`;;
+
+let arm_UBFM = define
+ `arm_UBFM Rd Rn immr imms =
+    \s. let x:N word = read Rn (s:armstate) in
+        let y:N word =
+          if imms >= immr then word_subword x (immr,(imms-immr)+1)
+          else word_shl (word_subword x (0,imms+1)) (dimindex(:N) - immr) in
+        (Rd := y) s`;;
 
 let arm_UMULH = define
  `arm_UMULH Rd Rn Rm =
@@ -1018,6 +1051,9 @@ let arm_BLE = define `arm_BLE = arm_Bcond Condition_LE`;;
 let arm_BAL = define `arm_BAL = arm_Bcond Condition_AL`;;
 let arm_BNV = define `arm_BNV = arm_Bcond Condition_NV`;;
 
+let arm_CINC = define
+ `arm_CINC Rd Rn cc = arm_CSINC Rd Rn Rn (invert_condition cc)`;;
+
 let arm_CINV = define
  `arm_CINV Rd Rn cc = arm_CSINV Rd Rn Rn (invert_condition cc)`;;
 
@@ -1033,22 +1069,12 @@ let arm_CSET = define
 let arm_CSETM = define
   `arm_CSETM Rd cc = arm_CSINV Rd ZR ZR (invert_condition cc)`;;
 
-(*** ARM actually aliases most/all immediate shifts LSL LSR to UBFM.
- *** But in our setting it seems much simpler to use LSLV and LSRV directly.
- *** I assume the semantics must be the same, though I didn't trace
- *** through the instances of UBFM.
- ***)
-
-let arm_LSL = define
- `arm_LSL Rd Rm Rn = arm_LSLV Rd Rm Rn`;;
-
-let arm_LSR = define
- `arm_LSR Rd Rm Rn = arm_LSRV Rd Rm Rn`;;
-
 let arm_MOV = define `arm_MOV Rd Rm = arm_ORR Rd ZR Rm`;;
 
 let arm_MNEG = define `arm_MNEG Rd Rn Rm = arm_MSUB Rd Rn Rm ZR`;;
 let arm_MUL = define `arm_MUL Rd Rn Rm = arm_MADD Rd Rn Rm ZR`;;
+
+let arm_MVN = define `arm_MVN Rd Rm = arm_ORN Rd ZR Rm`;;
 
 let arm_NEG = define `arm_NEG Rd Rm = arm_SUB Rd ZR Rm`;;
 let arm_NEGS = define `arm_NEGS Rd Rm = arm_SUBS Rd ZR Rm`;;
@@ -1064,27 +1090,73 @@ let ARM_INSTRUCTION_ALIASES =
  [arm_BEQ; arm_BNE; arm_BCS; arm_BHS; arm_BCC;
   arm_BLO; arm_BMI; arm_BPL; arm_BVS; arm_BVC;
   arm_BHI; arm_BLS; arm_BGE; arm_BLT; arm_BGT;
-  arm_BLE; arm_BAL; arm_BNV; arm_CMN; arm_CMP;
-  arm_CINV; arm_CNEG; arm_CSET; arm_CSETM;
-  arm_LSL; arm_LSR; arm_MOV; arm_MNEG; arm_MUL;
-  arm_NEG; arm_NEGS; arm_NGC; arm_NGCS; arm_ROR;
-  arm_TST];;
+  arm_BLE; arm_BAL; arm_BNV; arm_CINC; arm_CINV; 
+  arm_CNEG; arm_CMN; arm_CMP;arm_CSET; arm_CSETM; 
+  arm_MOV; arm_MNEG; arm_MUL; arm_MVN; arm_NEG; 
+  arm_NEGS; arm_NGC; arm_NGCS; arm_ROR; arm_TST];;
+
+(* ------------------------------------------------------------------------- *)
+(* These two are treated by ARM as aliases, but since they are such          *)
+(* natural top-level operations we define them a priori then prove           *)
+(* they are equivalent to their UBFM instances given some sideconditions.    *)
+(* The decoder will return them directly instead of expanding to UBFM.       *)
+(*                                                                           *)
+(* Note that you can't actually encode a left shift by zero bits; it         *)
+(* is instead interpreted as a right shift by zero bits. However the alias   *)
+(* arm_LSL with a zero shift does in fact mean the same thing anyway.        *)
+(* ------------------------------------------------------------------------- *)
+
+let arm_LSL = define
+ `arm_LSL Rd Rn imm =
+        \s. let x:N word = read Rn (s:armstate) in
+            let y = word_shl x imm in
+            (Rd := y) s`;;
+
+let arm_LSR = define
+ `arm_LSR Rd Rn imm =
+       \s. let x:N word = read Rn (s:armstate) in
+           let y = word_ushr x imm in
+           (Rd := y) s`;;
+
+let arm_LSL_ALIAS = prove
+ (`immr < dimindex(:N) /\ imms + 1 = immr
+   ==> arm_UBFM (Rd:(armstate,N word)component) Rn immr imms =
+       arm_LSL Rd Rn (dimindex(:N) - immr)`,
+  DISCH_THEN(CONJUNCTS_THEN2 ASSUME_TAC (SUBST1_TAC o SYM)) THEN
+  GEN_REWRITE_TAC I [FUN_EQ_THM] THEN
+  X_GEN_TAC `s:armstate` THEN ASM_REWRITE_TAC[arm_LSL; arm_UBFM] THEN
+  LET_TAC THEN CONV_TAC(TOP_DEPTH_CONV let_CONV) THEN
+  AP_THM_TAC THEN AP_TERM_TAC THEN REWRITE_TAC[ARITH_RULE `~(s >= s + 1)`] THEN
+  ASM_SIMP_TAC[MOD_CASES; DIMINDEX_GE_1; ARITH_RULE `1 <= n ==> n - d < 2 * n`;
+               ARITH_RULE `1 <= n ==> (n - d < n <=> ~(d = 0))`] THEN
+  SIMP_TAC[COND_SWAP; SUB_0; SUB_REFL; GE] THEN
+  ASM_CASES_TAC `imm = 0` THEN
+  ASM_SIMP_TAC[LE_0; SUB_0; SUB_ADD; DIMINDEX_GE_1; GSYM WORD_ZX_SUBWORD;
+               WORD_ZX_TRIVIAL; WORD_SHL_ZERO] THEN
+  ASM_SIMP_TAC[ARITH_RULE `d < n ==> ~(n - d <= n - 1 - d)`] THEN
+  ASM_SIMP_TAC[ARITH_RULE `d:num < n ==> n - (n - d) = d`] THEN
+  ASM_SIMP_TAC[ARITH_RULE `d < n ==> n - 1 - d + 1 = n - d`] THEN
+  MATCH_MP_TAC WORD_SHL_SUBWORD THEN ARITH_TAC);;
+
+let arm_LSR_ALIAS = prove
+ (`immr < dimindex(:N) /\ imms = dimindex(:N) - 1
+   ==> arm_UBFM (Rd:(armstate,N word)component) Rn immr imms =
+       arm_LSR Rd Rn immr`,
+  REPEAT STRIP_TAC THEN GEN_REWRITE_TAC I [FUN_EQ_THM] THEN
+  X_GEN_TAC `s:armstate` THEN ASM_REWRITE_TAC[arm_LSR; arm_UBFM] THEN
+  LET_TAC THEN CONV_TAC(TOP_DEPTH_CONV let_CONV) THEN
+  AP_THM_TAC THEN AP_TERM_TAC THEN
+  ASM_SIMP_TAC[ARITH_RULE `d < n ==> n - 1 >= d`] THEN
+  ASM_SIMP_TAC[ARITH_RULE `d < n ==> n - 1 - d + 1 = n - d`] THEN
+  REWRITE_TAC[WORD_USHR_AS_SUBWORD]);;
 
 (* ------------------------------------------------------------------------- *)
 (* The ROR alias does amount to the same thing as the word_ror operation.    *)
 (* ------------------------------------------------------------------------- *)
 
-(**** We wire in 64-bit words here, but it would work with the shift
- **** being a 6-bit immediate as well
- ****)
-
 let arm_ROR_ALT = prove
  (`arm_ROR Rd Rs lsb =
-    \s:armstate.
-          let n:64 word = read Rs s
-          and l:64 word = read lsb s in
-          let d = word_ror n (val l) in
-          (Rd := d) s`,
+    \s:armstate. (Rd := word_ror (read Rs s) lsb) s`,
   GEN_REWRITE_TAC I [FUN_EQ_THM] THEN X_GEN_TAC `s:armstate` THEN
   REWRITE_TAC[arm_ROR; arm_EXTR] THEN
   CONV_TAC(TOP_DEPTH_CONV let_CONV) THEN
@@ -1256,14 +1328,19 @@ let arm_MOVK_ALT =
 
 let ARM_OPERATION_CLAUSES =
   map (CONV_RULE(TOP_DEPTH_CONV let_CONV) o SPEC_ALL)
-      [arm_ADC; arm_ADCS_ALT; arm_ADD; arm_ADDS_ALT;
-       arm_AND; arm_ANDS; arm_B; arm_BL; arm_BL_ABSOLUTE; arm_Bcond;
+      [arm_ADC; arm_ADCS_ALT; arm_ADD; arm_ADDS_ALT; arm_AND; arm_ANDS;
+       arm_ASRV; arm_B; arm_BIC; arm_BICS; arm_BL; arm_BL_ABSOLUTE; arm_Bcond;
        arm_CBNZ_ALT; arm_CBZ_ALT; arm_CLZ; arm_CSEL; arm_CSINC;
-       arm_CSINV; arm_CSNEG; arm_EON; arm_EOR; arm_EXTR; arm_LSLV;
-       arm_LSRV; arm_MOVK_ALT; arm_MOVN; arm_MOVZ;
-       arm_MADD; arm_MSUB; arm_ORN;
-       arm_ORR; arm_RET; arm_SBC; arm_SBCS_ALT;
-       arm_SUB; arm_SUBS_ALT; arm_UMULH];;
+       arm_CSINV; arm_CSNEG; arm_EON; arm_EOR; arm_EXTR;
+       arm_LSL; arm_LSLV; arm_LSR; arm_LSRV;
+       arm_MADD; arm_MOVK_ALT; arm_MOVN; arm_MOVZ;
+       arm_MSUB; arm_ORN; arm_ORR; arm_RET; arm_RORV; arm_SBC; arm_SBCS_ALT;
+       arm_SUB; arm_SUBS_ALT; arm_UBFM; arm_UMULH;
+    (*** 32-bit backups since the ALT forms are 64-bit only ***)
+       INST_TYPE[`:32`,`:N`] arm_ADCS;
+       INST_TYPE[`:32`,`:N`] arm_ADDS;
+       INST_TYPE[`:32`,`:N`] arm_SBCS;
+       INST_TYPE[`:32`,`:N`] arm_SUBS];;
 
 let ARM_LOAD_STORE_CLAUSES =
   map (CONV_RULE(TOP_DEPTH_CONV let_CONV) o SPEC_ALL)
